basic_step_simrel_a2e_h lemma refactoring

Coq/src/SimRelCertBasicStep.v
@@ -111,22 +111,38 @@ Section SimRelCertBasicStep.
   Notation "'cont_lang'" :=
     (fun S k => thread_lts (ES.cont_thread S k)) (at level 10, only parsing).
 
-  Lemma basic_step_simrel_a2e_h k k' e e' S S' 
+  Definition upd_a2e a2e e e' S' := 
+    upd_opt (upd a2e (e2a S' e) e) (option_map (e2a S') e') e'.
+
+  Lemma basic_step_simrel_updh_cert_dom_eq_dom k k' e e' S S' 
         (st st' st'': thread_st (ES.cont_thread S k))
         (SRCC : simrel_cert prog S G sc TC TC' f h k st st'')
         (BSTEP_ : ESBasicStep.t_ (cont_lang S k) k k' st st' e e' S S') : 
-    let h' := upd_opt (upd h (e2a S' e) e) (option_map (e2a S') e') e' in 
-    simrel_a2e S' h' (cert_dom G TC (ES.cont_thread S' k') st'). 
+    eq_dom (cert_dom G TC (ES.cont_thread S k) st) (upd_a2e h e e' S') h.
   Proof. 
-    cdes BSTEP_. 
-    assert (ESBasicStep.t e e' S S') as BSTEP.
-    { econstructor. eauto. }
+    red. ins. unfold upd_a2e.
+    rewrite updo_opt; auto.
+    { rewrite updo; auto. 
+      red. ins. subst. 
+      eapply basic_step_cert_dom_ne;
+        try apply SRCC; eauto. }
+    { unfold eq_opt, option_map. 
+      destruct e'; try done.
+      red; ins; subst.
+      eapply basic_step_cert_dom_ne';
+        try apply SRCC; eauto. }
+    apply option_map_same_ctor.
+  Qed.
 
-    set (h' := upd_opt (upd h (e2a S' e) e) (option_map (e2a S') e') e').
-
-    assert 
-      (~ eq_opt (option_map (e2a S') e') (e2a S' e))
-      as NEQe'.
+  Lemma basic_step_simrel_updh_e k k' e e' S S' 
+        (st st' st'': thread_st (ES.cont_thread S k))
+        (SRCC : simrel_cert prog S G sc TC TC' f h k st st'')
+        (BSTEP_ : ESBasicStep.t_ (cont_lang S k) k k' st st' e e' S S') : 
+    (upd_a2e h e e' S') (e2a S' e) = e.
+  Proof. 
+    unfold upd_a2e. 
+    rewrite updo_opt.
+    { by rewrite upds. }
     { unfold eq_opt.
       destruct e' as [e'|]; simpl; red; ins.
       erewrite basic_step_e2a_e with (e := e) in H; eauto.
@@ -134,112 +150,109 @@ Section SimRelCertBasicStep.
       erewrite basic_step_e2a_e' in H; eauto.
       2-5 : apply SRCC.
       inv H. omega. }
+    apply option_map_same_ctor.
+  Qed.
 
-    assert 
-      (set_disjoint (eq (e2a S' e)) (eq_opt (option_map (e2a S') e'))) 
-      as DISJe'.
-    { unfold eq_opt.
-      destruct e'; simpl; red; ins.
-      erewrite basic_step_e2a_e in IN; eauto.
-      2-5 : apply SRCC.
-      erewrite basic_step_e2a_e' in IN'; eauto.
-      2-5 : apply SRCC.
-      inv IN. omega. }
+  Lemma basic_step_simrel_updh_e' k k' e e' S S' 
+        (st st' st'': thread_st (ES.cont_thread S k))
+        (SRCC : simrel_cert prog S G sc TC TC' f h k st st'')
+        (BSTEP_ : ESBasicStep.t_ (cont_lang S k) k k' st st' e e' S S') : 
+    option_map (upd_a2e h e e' S') (option_map (e2a S') e') = e'.
+  Proof.
+    destruct e' as [e'|]; auto.
+    unfold upd_a2e, option_map, upd_opt.
+    by rewrite upds.
+  Qed.
 
-    assert 
-      (opt_same_ctor (option_map (e2a S') e') e') 
-      as CTORe'.
-    { unfold opt_same_ctor, option_map. by destruct e'. }
+  Lemma basic_step_simrel_updh_cert_dom k k' e e' S S' 
+        (st st' st'': thread_st (ES.cont_thread S k))
+        (SRCC : simrel_cert prog S G sc TC TC' f h k st st'')
+        (BSTEP_ : ESBasicStep.t_ (cont_lang S k) k k' st st' e e' S S') : 
+    upd_a2e h e e' S' □₁ (cert_dom G TC (ES.cont_thread S' k') st') ≡₁
+            h □₁ (cert_dom G TC (ES.cont_thread S k) st) ∪₁ eq e ∪₁ eq_opt e'. 
+  Proof. 
+    erewrite basic_step_cert_dom; 
+      eauto; try apply SRCC.
+    rewrite !set_collect_union.
+    repeat apply set_union_Propere.
+    { apply set_collect_eq_dom.
+      eapply basic_step_simrel_updh_cert_dom_eq_dom; eauto. }
+    { rewrite set_collect_eq.
+      erewrite basic_step_simrel_updh_e; eauto. }
+    rewrite set_collect_eq_opt.
+    erewrite basic_step_simrel_updh_e'; eauto.
+  Qed.
+    
+  Lemma basic_step_simrel_a2e_h k k' e e' S S' 
+        (st st' st'': thread_st (ES.cont_thread S k))
+        (SRCC : simrel_cert prog S G sc TC TC' f h k st st'')
+        (BSTEP_ : ESBasicStep.t_ (cont_lang S k) k k' st st' e e' S S') : 
+    simrel_a2e S' (upd_a2e h e e' S') (cert_dom G TC (ES.cont_thread S' k') st'). 
+  Proof. 
+    cdes BSTEP_. 
+    assert (ESBasicStep.t e e' S S') as BSTEP.
+    { econstructor. eauto. }
 
-    assert 
-      (eq_dom (cert_dom G TC (ES.cont_thread S k) st) h' h)
-      as EQhCERTD.
-    { red. ins. subst h'. 
-      rewrite updo_opt; auto.
-      2 : 
-        unfold eq_opt, option_map; 
-        destruct e'; try done;
-        red; ins; subst;
-        eapply basic_step_cert_dom_ne';
-        try apply SRCC; eauto. 
-      rewrite updo; auto. 
-      red. ins. subst. 
-      eapply basic_step_cert_dom_ne;
-        try apply SRCC; eauto. }
-
-    simpl. 
-    eapply simrel_a2e_set_equiv; try apply SRCC.
-    { eapply basic_step_cert_dom; eauto; apply SRCC. }
-    subst h'. constructor.
+    constructor.
     
     (* a2e_inj *)
-    { rewrite set_unionA.
-      eapply inj_dom_union.
-      { red. ins.
-        rewrite !EQhCERTD in EQ; auto.
+    { eapply inj_dom_more.
+      { eapply basic_step_cert_dom; eauto; apply SRCC. }
+      all : eauto.
+      rewrite set_unionA.
+      eapply inj_dom_union. 
+      { red. ins. 
+        erewrite !basic_step_simrel_updh_cert_dom_eq_dom 
+          in EQ; eauto.
         eapply a2e_inj; eauto. apply SRCC. }
-      { eapply inj_dom_union.
+      { apply inj_dom_union. 
         { apply inj_dom_eq. }
         { apply inj_dom_eq_opt. }
-        unfold option_map, eq_opt, upd_opt.
-        destruct e'; [|basic_solver].
-        rewrite !set_collect_eq.
-        rewrite updo, !upds; auto. 
-        basic_solver. }
-      erewrite set_collect_eq_dom; eauto.
+        rewrite set_collect_eq, set_collect_eq_opt.
+        erewrite basic_step_simrel_updh_e; eauto.
+        erewrite basic_step_simrel_updh_e'; eauto.
+        ESBasicStep.step_solver. }
+      erewrite set_collect_eq_dom.
+      2 : eapply basic_step_simrel_updh_cert_dom_eq_dom; eauto.
       rewrite set_collect_union.
-      rewrite set_collect_eq.
-      rewrite updo_opt; auto.
-      rewrite upds.
+      rewrite set_collect_eq, set_collect_eq_opt.
+      erewrite basic_step_simrel_updh_e; eauto.
+      erewrite basic_step_simrel_updh_e'; eauto.
       red. ins. destruct IN' as [IN' | IN'].
       { eapply ESBasicStep.basic_step_acts_set_ne; eauto.
         subst. eapply a2e_img; eauto. apply SRCC. }
       unfold eq_opt, option_map, upd_opt in IN'.
-      destruct e' as [e'|]. 
-      2 : { unfolder in IN'. by desc. }
-      apply set_collect_eq in IN'.
-      rewrite upds in IN'.
+      destruct e' as [e'|]; auto. 
       eapply ESBasicStep.basic_step_acts_set_ne'; eauto.
       subst. eapply a2e_img; eauto. apply SRCC. }
         
     (* a2e_img *)
-    { rewrite !set_collect_union.
-      rewrite !set_subset_union_l.
-      splits.
-      { erewrite set_collect_eq_dom; eauto.
-        rewrite a2e_img; try apply SRCC.
-        eapply ESBasicStep.basic_step_acts_set_mon; eauto. }
-      { rewrite set_collect_updo_opt; auto. 
-        rewrite set_collect_eq.
-        rewrite upds; auto.  
-        erewrite ESBasicStep.basic_step_acts_set; eauto. 
-        basic_solver. }
-      unfold upd_opt, option_map, eq_opt. 
-      destruct e'; [|basic_solver]. 
-      rewrite set_collect_eq.
-      rewrite upds.
-      erewrite ESBasicStep.basic_step_acts_set; eauto. 
-      basic_solver. }
+    { erewrite basic_step_simrel_updh_cert_dom; eauto.
+      rewrite a2e_img; try apply SRCC.
+      erewrite ESBasicStep.basic_step_acts_set
+        with (S' := S'); eauto. }
 
     (* a2e_fix *)
-    rewrite !fixset_union. splits. 
-    { eapply fixset_eq_dom.
+    { eapply fixset_more.
+      { eapply basic_step_cert_dom; eauto; apply SRCC. }
+      all : eauto.
+      rewrite !fixset_union. splits. 
+      { eapply fixset_eq_dom.
+        { unfold eq_dom, compose. 
+          intros x DOM.
+          erewrite basic_step_simrel_updh_cert_dom_eq_dom; eauto.
+          erewrite basic_step_e2a_eq_dom; eauto.
+          { by fold (compose (e2a S) h x). }
+          { apply SRCC. }
+          apply SRCC.(sr_a2e_h).
+          basic_solver. }
+        apply SRCC. }
       { unfold eq_dom, compose. 
-        intros x DOM.
-        rewrite EQhCERTD; auto.
-        erewrite basic_step_e2a_eq_dom; eauto.
-        { by fold (compose (e2a S) h x). }
-        { apply SRCC. }
-        apply SRCC.(sr_a2e_h).
-        basic_solver. }
-      apply SRCC. }
-    { unfold eq_dom, compose. 
-      intros x DOM. subst x. 
-      rewrite updo_opt; auto. 
-      by rewrite upds. }
-    unfold eq_opt, option_map, upd_opt. 
-    red. ins. destruct e'; [|by exfalso].
-    unfold compose. subst x. by rewrite upds. 
+        intros x DOM. subst x. 
+        erewrite basic_step_simrel_updh_e; eauto. }
+      unfold upd_a2e, eq_opt, option_map, upd_opt. 
+      red. ins. destruct e'; [|by exfalso].
+      unfold compose. subst x. by rewrite upds. }
 
     all : admit. 
   Admitted.
@@ -265,7 +278,7 @@ Section SimRelCertBasicStep.
   Proof. 
     cdes BSTEP_. 
     constructor.
-    (* cstate_stable : stable_state (ES.cont_thread S' k') st''; *)
+    (* cstate_stable : stable_state (ES.cont_thread S' k') st'' *)
     { erewrite ESBasicStep.basic_step_cont_thread_k; eauto.
       eapply cstate_stable. apply SRCC. }
     (* cstate_q_cont : Kstate (k', st'); *)
